HashTable/hashtbl_proof_manual.v
@@ -115,13 +115,13 @@ Proof.
     sep_apply PtrArray.missing_i_merge_to_full.
     sep_apply (ptr_string_name i_v i_v_key k_list_current).
     2: { lia. }
-    2: { subst k_list_current. apply H7. }
+    2: { subst k_list_current. apply H11. }
     unfold store_hash_skeleton.
-    sep_apply (store_map_merge store_name k_list_current i_v m H7).
+    sep_apply (store_map_merge store_name k_list_current i_v m H11).
     pose (lh' := replace_Znth ind i_v lh).
     pose (b0' := update_b0_at b0 ind i_v lh').
     Exists l lh' b0' h_bucks.
-    assert (NULL = 0). {reflexivity. } rewrite H20.
+    assert (NULL = 0). {reflexivity. } rewrite H24.
     assert (NBUCK = 211). {reflexivity. }
     unfold lh'. 
     entailer!.
@@ -131,7 +131,7 @@ Admitted.
 Lemma proof_of_hashtbl_findref_return_wit_2 : hashtbl_findref_return_wit_2.
 Proof. Admitted. 
 
-Lemma proof_of_hashtbl_findref_partial_solve_wit_5_pure : hashtbl_findref_partial_solve_wit_5_pure.
+Lemma proof_of_hashtbl_findref_return_wit_3 : hashtbl_findref_return_wit_3.
 Proof. Admitted. 
 
 Lemma proof_of_hashtbl_findref_which_implies_wit_1 : hashtbl_findref_which_implies_wit_1.
@@ -146,10 +146,38 @@ Qed.
 Lemma proof_of_hashtbl_findref_which_implies_wit_2 : hashtbl_findref_which_implies_wit_2.
 Proof. 
     pre_process.
-Admitted. 
+    unfold contain_all_correct_addrs in H2.
+    pose proof H2 i_v ind; destruct H4.
+    rewrite (sll_head i_v l_res H).
+    Intros l_resres.
+    destruct H5. { exists (Znth ind lh 0), l0. split; [apply H1 | ]. rewrite H3. rewrite H6. apply in_elt. }
+    destruct H5.
+    sep_apply (store_map_split store_name x i_v m H5).
+    unfold store_name at 2.
+    Intros i_v_key.
+    subst l_res.
+    simpl.
+    Intros i_v_next.
+    Exists i_v_key i_v_next l_resres x.
+    entailer!.
+Qed.
 
-Lemma proof_of_hashtbl_findref_which_implies_wit_3 : hashtbl_findref_which_implies_wit_3.
-Proof. Admitted. 
+Lemma proof_of_hashtbl_findref_which_implies_wit_4 : hashtbl_findref_which_implies_wit_4.
+Proof. 
+    pre_process.
+    destruct l_prev.
+    + rewrite <-derivable1_orp_intros1.
+        simpl.
+        entailer!.
+        rewrite H.
+        rewrite H0.
+        entailer!.
+    + rewrite <- derivable1_orp_intros2.
+        Exists z l_prev.
+        entailer!.
+        simpl.
+        entailer!.
+Qed. 
 
 Lemma proof_of_hashtbl_remove_entail_wit_1 : hashtbl_remove_entail_wit_1.
 Proof. pre_process.
